correctness/RegexCorrectness/Regex/OptimizationInfo.lean
@@ -1,0 +1,41 @@
+import Regex.Regex.OptimizationInfo
+import RegexCorrectness.Data.Expr.Semantics
+import RegexCorrectness.Data.Expr.Optimization
+import RegexCorrectness.Data.String
+
+open Regex.Data (Expr CaptureGroups)
+open String (Iterator)
+
+namespace Regex.OptimizationInfo
+
+@[simp, grind =]
+theorem findStart_toString {it : Iterator} {opt : OptimizationInfo} : (opt.findStart it).toString = it.toString := by
+  unfold findStart
+  grind
+
+theorem findStart_le_pos {it : Iterator} {opt : OptimizationInfo} : it.pos ≤ (opt.findStart it).pos := by
+  fun_cases findStart opt it
+  next => exact Iterator.find_le_pos
+  next => exact Nat.le_refl _
+
+theorem valid_findStart_of_valid {it : Iterator} {opt : OptimizationInfo} (v : it.Valid) : (opt.findStart it).Valid := by
+  fun_cases findStart opt it
+  next => exact Iterator.find_valid_of_valid v
+  next => exact v
+
+theorem findStart_completeness {it it' it'' : Iterator} {opt : OptimizationInfo} {groups : CaptureGroups} {e : Expr}
+  (eq : opt = .fromExpr e) (v : it.Valid) (eqs : it'.toString = it.toString) (ge : it.pos ≤ it'.pos)
+  (lt : it'.pos < (opt.findStart it).pos) (c : e.Captures it' it'' groups) :
+  False := by
+  revert lt
+  fun_cases findStart opt it
+  next ch h =>
+    intro lt
+    have ne := Iterator.find_completeness v it' c.validL eqs ge lt
+    simp at ne
+    simp [eq, fromExpr] at h
+    have eq : it'.curr = ch := Expr.curr_of_captures_of_firstChar_some c h
+    exact ne eq
+  next => exact Nat.not_lt_of_ge ge
+
+end Regex.OptimizationInfo
